\documentclass[letterpage]{article}
\usepackage{amsmath}
\usepackage{amssymb}


\begin{document}
\begin{align}
  g(x)&=e^{-a(x-b)^2}\\
  \frac{dg(x)}{dx}& = -2a(x-b)g(x)
\end{align}
Fourier transform pair is defined to be,
\begin{equation}
  G(w) = F\{g(x)\} = \int_{-\infty}^\infty g(x)e^{iwx}dx
\end{equation}
Then,
\begin{equation}
  \frac{dG(w)}{dw} = \int_{-\infty}^\infty ixg(x)e^{iwx}dx = F\{ixg(x)\}
\end{equation}
Taking the Fourier transform of both sides of (1), we get
\begin{align}
  -iwG(w) &= -2a \left(\frac{1}{i} \frac{dG(w)}{dw} - bG(w)\right)\\
  \left(ib-\frac{w}{2a}\right) G(w) &= \frac{dG(w)}{dw} \Rightarrow
  \frac{1}{G(w)} \frac{dG(w)}{dw} = ib-\frac{w}{2a}\\
  \int_0^w \frac{1}{G(w)'} \frac{dG(w)'}{dw'} dw' &= 
  \arrowvert\ln G(w')\arrowvert_0^w = \ln G(w) - \ln G(0) 
  = \ln \frac{G(w)}{G(0)}\\
  \int_0^w \left(ib-\frac{w}{za}\right)dw' &= \arrowvert ibw' - \frac{{w'}^2}{-4a}
  \arrowvert_0^w = ibw-\frac{w^2}{4a}\\
  G(0) = \int_{-\infty}^\infty g(x) dx &= \int_{-\infty}^\infty e^{-a(x-b)^2}
  = \sqrt{\frac{\pi}{a}}
\end{align}
From (2), (3), and (4), we get
\begin{align}
  G(w) = G(0) e^{ibw-\frac{w^2}{4a}} &= \sqrt{\frac{\pi}{a}} \quad e^{ibw} 
  e^{-\frac{w^2}{4a}}\\
  \text{or} \qquad
  \int_{-\infty}^\infty e^{-a(x-b)^2} e^{iqx}dx &= \sqrt{\frac{\pi}{a}}
  \quad e^{ibq} e^{-\frac{q^2}{4a}}
\end{align}
\begin{align}
  g(x) &= F^{-1} \{G(w)\} = \frac{1}{2\pi} \int_{-\infty}^\infty 
  G(w)e^{-iwx}dw\\
  \text{and} \qquad \frac{dg(x)}{dx} &= \frac{1}{2\pi} \int_{-\infty}^\infty
  (-iw)G(w)e^{-iwx}dw\\
  &=F^{-1} \left\{-iwG(w)\right\}\\
  &\Rightarrow F\left\{\frac{dg(x)}{dx} \right\} = -(iwG(w))
\end{align}
\\
\begin{equation*}
  u(x) = 
    \begin{cases}
    -\frac{A}{\lambda_r - X_0} \left(x+\frac{\lambda_r}{2}\right) 
     &\text{ for } 
    -\frac{\lambda_r}{2} \leq x < -\frac{x_0}{2}\\
    \quad \frac{A}{x_0}x &\text{ for } 
    -\frac{x_0}{2} \leq x \leq \frac{x_0}{2}\\
    -\frac{A}{\lambda_r-X_0} \left(x-\frac{\lambda_r}{2}\right)
    &\text{ for } 
   \frac{x_0}{2} < x \leq \frac{\lambda_r}{2}
    \end{cases}
\end{equation*}
\begin{align}
  Fc(\textbf{q}) &= \int_{-\frac{\lambda_r}{2}}^{\frac{\lambda_r}{2}}dx
  \int_{-\frac{D}{2}}^\frac{D}{2} dz \quad \delta\left(z-u(x)\right)
  e^{iq_zZ} e^{iq_xX} \\
  &= \int_{\frac{-\lambda_r}{2}}^{\frac{\lambda_r}{2}} dx \quad e^{iq_zu(x)}
  e^{iq_xX}
\end{align}
\begin{align}
  \int_{-\frac{\lambda_r}{2}}^{-\frac{x_0}{2}} dx \quad e^{iq_xx} e^{iq_zu(x)}
  &= -\int_{\frac{\lambda_r}{2}}^{\frac{x_0}{2}} 
  dy \quad e^{-iq_xy}e^{iq_zu(-y)}\\
  &= \int_{\frac{x_0}{2}}^{\frac{\lambda_r}{2}} dx \quad e^{-iq_xx} 
  e^{iq_z\frac{A}{\lambda_r-x_0}\left(x-\frac{\lambda_r}{2}\right)}\\
  &= \int_{\frac{x_0}{2}}^{\frac{\lambda_r}{2}}dx \quad 
  e^{-i\left[q_xx - q_z \frac{A}{\lambda_r-x_0}
  \left(x-\frac{\lambda_r}{2}\right)\right]}
\end{align}
\end{document}